cminusP generic

abstract_montgomery_ladder/Abstract_exp_proof_1.ec
@@ -15,12 +15,17 @@ op Rsize : int.
 op valR (x : R) : int.
 op of_int (x : int) : R.
 
+op idR : R.
+op ( ** ) : int -> int -> int.
+
+op ( *** ) (a b : R) : R. (* = of_int ((valR a ** valR b) %% P). *)
+
 op Rbits (r : R) : bits = int2bs Rsize (valR r).
 op bitsR (r : bits) : R = of_int (bs2int r).
 
 module type BasicOps = {
   proc ith_bit (r : R, p : W64.t) : W64.t
-  proc mulm (p : R, a : R, b : R) : R
+  proc opr (p : R, a : R, b : R) : R
   proc swapr (a : R, b : R, c : W64.t) : R * R
 }.
 
@@ -34,16 +39,8 @@ op as_w64 (x : bool) : W64.t  = x ? W64.one : W64.zero.
 op ith_bitR (r : R) (x : int) : W64.t = as_w64 (ith_bit (Rbits r) x).
 op as_bool (x : W64.t) : bool  = (x = W64.one).
 op ith_bitlist (n : bits) (x : int)  : W64.t = as_w64 (ith_bit n x).
-(* op valR (x : R) : int = bs2int (Rbits x). *)
-(* op of_int (x : int) : R = bitsR (int2bs Rsize x). *)
 op ImplR (p : R) (P : int) = (valR p = P).
-
-op oneR : R = of_int 1.
-
-op ( *** ) (a b : R) : R = of_int (valR a * valR b %% P).
-
-
-op (^) (x : R) (n : int) : R = if n < 0 then iterop (-n) ( *** ) x oneR else iterop n ( *** ) x oneR.
+op (^) (x : R) (n : int) : R = if n < 0 then iterop (-n) ( *** ) x idR else iterop n ( *** ) x idR.
 
 
 lemma qqq n x : ith_bitlist (Rbits n) x = ith_bitR n x.
@@ -62,6 +59,12 @@ axiom valr_ofint x : 0 <= x < P => valR (of_int x) = x.
 axiom ofint_valr x : of_int (valR x) = x.
 axiom rbits_bitsr x : size x = Rsize => Rbits (bitsR x) = x.
 axiom bitsr_rbits x : bitsR (Rbits x) = x.
+axiom exp_prop7 (a b : R) :  a *** b = b *** a.
+axiom exp_prop6 (a b c : R) :  (a *** b) *** c = a *** (b *** c).
+axiom exp_prop5 (x : R) : valR x < P => x *** idR = x. 
+axiom idR_leP :  valR idR < P.
+axiom mult_valr a b : valR (a *** b) < P.
+
 
 
 lemma mod_lemm (a b c m : int) : ((a * b %% m) * c) %% m = ((a * b) * c) %% m. 
@@ -69,30 +72,26 @@ smt (modzMml modzMm modzMmr).
 qed.
 
     
-lemma exp_prop7 (a b : R) :  a *** b = b *** a.
-proof. smt. qed.
+
+(* proof. rewrite /( *** ).   admitted. *)
+
+(* have ->: (valR ((of_int (valR a + valR b %% P))) + valR c %% P) *)
+(*   = (valR a + valR ((of_int (valR b + valR c %% P))) %% P). *)
+
+(*   have ->: valR ((of_int (valR a + valR b %% P))) = (valR a + valR b %% P). *)
+(*    smt. *)
+(*   have ->: ((valR a + valR b) %% P) + valR c %% P = ((valR a + valR b)  + valR c) %% P .  *)
+(*   smt (mod_lemm). *)
+(*   have ->: valR ((of_int (valR b + valR c %% P))) = valR b + valR c %% P. smt. *)
+(*   have ->: valR a + (valR b + valR c %% P) %% P = valR a + (valR b + valR c) %% P. smt (mod_lemm). *)
+(*   smt(). *)
+(*   auto. *)
+(* qed.  *)
 
 
-
-lemma exp_prop6 (a b c : R) :  (a *** b) *** c = a *** (b *** c).
-proof. rewrite /( *** ). 
-
-have ->: (valR ((of_int (valR a * valR b %% P))) * valR c %% P)
-  = (valR a * valR ((of_int (valR b * valR c %% P))) %% P).
-  have ->: valR ((of_int (valR a * valR b %% P))) = (valR a * valR b %% P).
-   smt.
-  have ->: ((valR a * valR b) %% P) * valR c %% P = ((valR a * valR b)  * valR c) %% P . 
-  smt (mod_lemm).
-  have ->: valR ((of_int (valR b * valR c %% P))) = valR b * valR c %% P. smt.
-  have ->: valR a * (valR b * valR c %% P) %% P = valR a * (valR b * valR c) %% P. smt (mod_lemm).
-  smt().
-  auto.
-qed. 
-
-
-lemma to_uintP: forall (x y : R), valR (x *** y) = valR x * valR y %% P.
-progress. rewrite /( *** ). smt.
-qed.
+(* lemma to_uintP: forall (x y : R), valR (x *** y) = (valR x ** valR y) %% P. *)
+(* progress. rewrite /( *** ). smt. *)
+(* qed. *)
 
 lemma bitsR_prop a b : bs2int a = valR b => size a = Rsize => bitsR a = b.
 proof. rewrite /valR.
@@ -108,29 +107,29 @@ rewrite /ith_bitlist. auto.
 smt(rbits_bitsr).
 qed.
 
-lemma valR_one : valR oneR = 1.
-rewrite /oneR. rewrite valr_ofint. auto.
-smt. auto.
-qed.
+(* lemma valR_one : valR idR = 0. *)
+(* rewrite /oneR. rewrite valr_ofint. auto. *)
+(* smt. auto. *)
+(* qed. *)
 
 
-lemma exp_prop5 (x : R) : valR x < P => x *** oneR = x. 
-progress. rewrite /( *** ). 
-have -> : valR oneR = 1. smt. simplify.
-have ->: (valR x %% P) = valR x. 
-have : 0 <= valR x. smt(valr_pos).
-smt.
-smt(ofint_valr).
-qed.
+
+(* progress. rewrite /( *** ).  *)
+(* have -> : valR idR = 0. smt. simplify. *)
+(* have ->: (valR x %% P) = valR x.  *)
+(* have : 0 <= valR x. smt(valr_pos). *)
+(* smt. *)
+(* smt(ofint_valr). *)
+(* qed. *)
 
 
 lemma iteropi : forall i, 0 <= i => forall  b, valR b < P =>
-  iterop (i + 1) ( *** ) b oneR = b *** iterop i ( *** ) b oneR.
+  iterop (i + 1) ( *** ) b idR = b *** iterop i ( *** ) b idR.
 apply intind.
 progress. 
- have ->: iterop 0 ( *** ) b oneR = oneR.
+ have ->: iterop 0 ( *** ) b idR = idR.
 smt(@IterOp).
-  have ->: iterop 1 ( *** ) b oneR = b.
+  have ->: iterop 1 ( *** ) b idR = b.
 smt(@IterOp).
 rewrite exp_prop5. auto.
 progress. progress.
@@ -165,7 +164,7 @@ apply bs2int_ge0.
 qed.
 
 
-lemma exp_prop1 x : x ^ 0 = oneR.
+lemma exp_prop1 x : x ^ 0 = idR.
 smt (@IterOp). qed.
 
 lemma exp_prop2 x : x ^ 1 = x.
@@ -175,11 +174,12 @@ smt (@IterOp). qed.
 
 
 
-lemma mult_valr a b : valR (a *** b)  < P.
-rewrite /( *** ).
-have : (valR a * valR b %% P) < P. smt.
-progress. smt. 
-qed.
+
+
+(* rewrite /( *** ). *)
+(* have : (valR a ** valR b %% P) < P. smt. *)
+(* progress. smt.  *)
+(* qed. *)
 
 
 
@@ -194,9 +194,10 @@ qed.
 
     
 
+
 lemma exp_valr x : forall i, 0 <= i => valR x < P =>  valR (x ^ i) < P.
 apply intind.
-progress. rewrite exp_prop1. smt.
+progress. rewrite exp_prop1. smt(idR_leP).
 progress. 
 have -> : i + 1 = 1 + i. smt().
 rewrite exp_prop3'. auto. auto.
@@ -204,11 +205,15 @@ smt(mult_valr).
 qed.
 
 lemma exp_prop3 (x : R) : forall (a : int), 0 <= a => forall b,  0 <= b => valR x < P => x ^ (a + b) = x ^ a *** x ^ b.
-apply intind. progress. rewrite exp_prop1.  smt (exp_prop5 exp_valr).
+apply intind. progress. rewrite exp_prop1.   smt (exp_prop7 exp_prop5 exp_valr).
 progress.
 have ->: (i + 1) = (1 + i). smt().
 have ->: x ^ (1 + i) = x *** x ^ i.
-smt (@IterOp).
+rewrite /(^).  
+have ->: 1 + i < 0 = false. smt(). simplify.
+have ->: i < 0 = false. smt(). simplify.
+have ->: 1 + i = i + 1. smt().
+rewrite iteropi. auto. auto. auto.
 rewrite exp_prop6.
 rewrite - H0. auto. auto.
 smt (exp_prop3').
@@ -227,7 +232,7 @@ smt (exp_prop7 exp_prop6).
 qed.
 
 
-lemma oner_exp : forall b, 0 <= b => oneR = oneR ^ b.
+lemma oner_exp : forall b, 0 <= b => idR = idR ^ b.
 apply intind. progress. smt(exp_prop1).
 progress. 
 have -> : (i+1) = 1 + i. smt().
@@ -252,20 +257,9 @@ rewrite exp_prop4'. auto. auto. smt (exp_valr). smt(exp_prop7).
 qed.
 
 
-(* Embedding into ring theory *)
-(* require ZModP. *)
-(* clone import ZModP.ZModField as Zp with *)
-(*         op p <= P *)
-(*         rename "zmod" as "zp" *)
-(*         proof prime_p by exact P_prime. *)
-
-(* op (^^) (x : zp)(n : int) : zp = inzp (asint x ^ n). *)
-
-(* abbrev ImplFp x y = valR x = asint y. *)
-
-
-op as_word (x : bool) : W64.t  = x ? W64.one : W64.zero.
-op ith_bitword64 (n : W64.t) (x : int)  : W64.t = as_word (n.[x]).
+require import Ith_Bit64.
+(* op as_word (x : bool) : W64.t  = x ? W64.one : W64.zero. *)
+(* op ith_bitword64 (n : W64.t) (x : int)  : W64.t = as_word (n.[x]). *)
 
 module Spec = {
   proc ith_bit(r : R, ctr : int) = {
@@ -284,18 +278,6 @@ module Spec = {
   proc swapr(a : R, b : R, c : bool) = {
     return c ? (b,a) : (a, b);
   }
-
- (* proc mulm(a b: zp): zp = { *)
- (*    var r; *)
- (*    r <- a * b; *)
- (*    return r; *)
- (* } *)
-
- (* proc expm(a : zp,  b: int): zp = { *)
- (*    var r; *)
- (*    r <- a ^^ b; *)
- (*    return r; *)
- (* } *)
 
 }.
 
@@ -319,7 +301,7 @@ lemma hast5  : forall xs, ! (has_true xs) => (bs2int xs) = 0.
 elim. smt. smt. qed.
 
 
-lemma hast4  : forall xs (x : R), ! (has_true xs) => x ^ (bs2int xs) = oneR.
+lemma hast4  : forall xs (x : R), ! (has_true xs) => x ^ (bs2int xs) = idR.
 progress. rewrite hast5. auto.
 rewrite /(^). simplify. smt.
 qed.
@@ -332,17 +314,17 @@ qed.
 
 module M1 = {
 
-  proc expm_spec (x:R, n:bits) : R = {
+  proc iterop_spec (x:R, n:bits) : R = {
     return x ^ (bs2int n); 
   }  
 
-  proc expm_naive (x:R, n:bits) : R = {
+  proc iterop_naive (x:R, n:bits) : R = {
     
     var x1, x2, x3, x4 : R;
     var ctr:int;
     var bit, d, p :bool;    
     d <- ith_bit n (size n - 1);
-    (x1,x2,x3, x4) <- (oneR,oneR,x,x *** x);
+    (x1,x2,x3, x4) <- (idR,idR,x,x *** x);
 
     ctr <- size n - 1;
     p <- d;
@@ -363,13 +345,13 @@ module M1 = {
 
 
 
-lemma exp_naive_correct xx nn : 
-  equiv[ M1.expm_naive ~ M1.expm_spec : ={arg} /\ arg{1} = (xx, nn){1}  /\  0 < size nn
+lemma iterop_spec_naive xx nn : 
+  equiv[ M1.iterop_naive ~ M1.iterop_spec : ={arg} /\ arg{1} = (xx, nn){1}  /\  0 < size nn
   /\ valR x{1} < P ==> ={res}].
 proof. proc. 
 while {1} (d{1} = has_true (drop ctr n) /\ ctr < size n /\ (has_true (drop ctr n) =>
   (x1 = x ^ bs2int (drop ctr n) 
-    /\ x2 = x1 *** x  /\ (x3,x4){1} = (oneR, oneR)) ) /\ (!has_true (drop ctr n) => x1 = oneR /\ x2 = oneR /\ x3 = x /\ x4 = x *** x) /\ valR x1 < P /\  valR x < P){1}   (ctr{1}). 
+    /\ x2 = x1 *** x  /\ (x3,x4){1} = (idR, idR)) ) /\ (!has_true (drop ctr n) => x1 = idR /\ x2 = idR /\ x3 = x /\ x4 = x *** x) /\ valR x1 < P /\  valR x < P){1}   (ctr{1}). 
 progress.
 wp. skip.  progress. 
 rewrite (drop_nth false (ctr{hr} - 1)). smt(). simplify. rewrite /ith_bit. smt().
@@ -409,13 +391,13 @@ pose n := bs2int (drop ctr{hr} n{hr}).
 smt (exp_prop6).
 pose n := bs2int (drop ctr{hr} n{hr}).
 rewrite exp_prop3. smt (prop5). auto. auto. rewrite exp_prop2.
-smt.
+have ->: (2 * n) = n + n. smt().
+rewrite exp_prop3. admit. admit. auto. auto.
 progress.
 have z: has_true (drop ctr{hr} n{hr}) = true. 
 have x : drop (ctr{hr} - 1) n{hr} = ith_bit n{hr} (ctr{hr} - 1) :: drop ctr{hr} n{hr}.
 rewrite (drop_nth false (ctr{hr} - 1)).  smt(). rewrite H6.
 simplify. rewrite - H6. rewrite /ith_bit. smt. smt.
-
 rewrite z.
 have -> : true ^ true  = false. smt(@Bool). simplify.
 have -> : x1{hr} *** x1{hr} = x{hr} ^ bs2int (drop ctr{hr} n{hr}) *** x{hr} ^ bs2int (drop ctr{hr} n{hr}).
@@ -430,32 +412,30 @@ simplify.
 case ( ith_bit n{hr} (ctr{hr} - 1)).
 progress. rewrite H0. auto.
 rewrite H0. auto. rewrite H0. auto.
-smt(exp_prop1 exp_prop2 exp_prop3 exp_prop4 exp_prop5 exp_prop6).
-smt(exp_prop1 exp_prop2 exp_prop3 exp_prop4 exp_prop5 exp_prop6).
+smt(exp_prop1 exp_prop2 exp_prop3 exp_prop4 exp_prop5 exp_prop6 exp_prop7).
+smt(exp_prop1 exp_prop2 exp_prop3 exp_prop4 exp_prop5 exp_prop6 exp_prop7).
 progress.
-smt(exp_prop1 exp_prop2 exp_prop3 exp_prop4 exp_prop5 exp_prop6).
+smt(exp_prop1 exp_prop2 exp_prop3 exp_prop4 exp_prop5 exp_prop6 exp_prop7).
 rewrite hast1. smt(). rewrite H5.
 case (has_true (drop ctr{hr} n{hr})).
 progress.
-smt(exp_prop1 exp_prop2 exp_prop3 exp_prop4 exp_prop5 exp_prop6).
-smt(exp_prop1 exp_prop2 exp_prop3 exp_prop4 exp_prop5 exp_prop6).
-
+smt(exp_prop1 exp_prop2 exp_prop3 exp_prop4 exp_prop5 exp_prop6 exp_prop7).
+smt(exp_prop1 exp_prop2 exp_prop3 exp_prop4 exp_prop5 exp_prop6 exp_prop7).
 rewrite hast1. smt(). rewrite H5.
 case (has_true (drop ctr{hr} n{hr})).
 progress.
-smt(exp_prop1 exp_prop2 exp_prop3 exp_prop4 exp_prop5 exp_prop6).
-smt(exp_prop1 exp_prop2 exp_prop3 exp_prop4 exp_prop5 exp_prop6).
-
+smt(exp_prop1 exp_prop2 exp_prop3 exp_prop4 exp_prop5 exp_prop6 exp_prop7).
+smt(exp_prop1 exp_prop2 exp_prop3 exp_prop4 exp_prop5 exp_prop6 exp_prop7).
 rewrite hast1. smt(). rewrite H5.
 case (has_true (drop ctr{hr} n{hr})).
 progress.
-smt(exp_prop1 exp_prop2 exp_prop3 exp_prop4 exp_prop5 exp_prop6).
-smt(exp_prop1 exp_prop2 exp_prop3 exp_prop4 exp_prop5 exp_prop6).
+smt(exp_prop1 exp_prop2 exp_prop3 exp_prop4 exp_prop5 exp_prop6 exp_prop7).
+smt(exp_prop1 exp_prop2 exp_prop3 exp_prop4 exp_prop5 exp_prop6 exp_prop7).
 rewrite hast1. smt(). rewrite H5.
 case (has_true (drop ctr{hr} n{hr})).
 progress.
-smt(exp_prop1 exp_prop2 exp_prop3 exp_prop4 exp_prop5 exp_prop6).
-smt(exp_prop1 exp_prop2 exp_prop3 exp_prop4 exp_prop5 exp_prop6).
+smt(exp_prop1 exp_prop2 exp_prop3 exp_prop4 exp_prop5 exp_prop6 exp_prop7).
+smt(exp_prop1 exp_prop2 exp_prop3 exp_prop4 exp_prop5 exp_prop6 exp_prop7).
 rewrite hast1. smt(). rewrite H5.
 smt.
 rewrite hast1. smt(). rewrite H5.
@@ -484,7 +464,7 @@ rewrite H3. auto.
 have -> : (drop ctr_L n{2}) = n{2}. smt.
 auto.
 progress.
-have -> : x1_L = oneR. smt. 
+have -> : x1_L = idR. smt. 
 have y : !has_true n{2}. smt. 
 rewrite  hast4. auto. auto.
 qed.
