abstract_montgomery_ladder/Abstract_exp_proof_3.ec
@@ -11,14 +11,13 @@ clone include Abstract_exp_proof_2.
 
 module M3 = {
 
-    proc expm (x:R, n:bits) : R = {
-    
+  proc iterop (x:R, n:bits) : R = {  
     var x1, x2, x3, x4, bit : R;
     var par, p, d : W64.t;
     var ctr:int;
 
     d <- ith_bitlist n (size n - 1);
-    (x1,x2,x3, x4) <- (oneR,oneR,x,x *** x);
+    (x1,x2,x3, x4) <- (idR,idR,x,x *** x);
 
     ctr <- size n - 1;
     p <- d;
@@ -39,22 +38,17 @@ module M3 = {
     (x1,x2) <- if ! as_bool (ith_bitlist n 0)  then (x2,x1) else (x1, x2);    
     return x1;
   }  
-
-
 }.
 
 
 
-lemma exp_2_3 :
- equiv[ M2.expm ~ M3.expm : ={arg} /\  0 < size n{1} ==> ={res}].
+lemma iterop_2_3 :
+ equiv[ M2.iterop ~ M3.iterop : ={arg} /\  0 < size n{1} ==> ={res}].
 proc.
 wp.
 while (={ctr, n,  x1,x2,  x3, x4}  
   /\ d{1} = as_bool d{2} /\ d{2} = as_w64 d{1} 
-  /\ p{1} = as_bool p{2} /\ p{2} = as_w64 p{1} 
-
-    )
-   .
+  /\ p{1} = as_bool p{2} /\ p{2} = as_w64 p{1}).
 wp. skip. progress. 
 timeout 20. smt.
 timeout 20. smt.
@@ -62,8 +56,6 @@ timeout 20. smt.
 timeout 20. smt.
 smt.
 smt.
-
-
 wp.  skip.  progress.
 smt.
 smt.
