abstract_montgomery_ladder/Abstract_exp_proof_8.ec
@@ -13,13 +13,13 @@ import IterOp.
 
 
 module M8 = {
-  proc expm_spec (x:R, n:R) : R = {
+  proc iterop_spec (x:R, n:R) : R = {
     return (x ^ (valR n));
   }  
 }.
 
-lemma exp_real_speac2 :
- equiv[ M8.expm_spec ~ M1.expm_spec   : arg{1}.`1 = arg{2}.`1 /\  valR arg{1}.`2 = bs2int arg{2}.`2 ==> ={res}] .
+lemma iterop_real_speac2 :
+ equiv[ M8.iterop_spec ~ M1.iterop_spec   : arg{1}.`1 = arg{2}.`1 /\  valR arg{1}.`2 = bs2int arg{2}.`2 ==> ={res}] .
 proc. skip. progress.
 smt().
 qed.
@@ -29,30 +29,30 @@ qed.
 section.
 declare module M <: BasicOps.
 
-declare axiom exp_swap :
+declare axiom iterop_swap :
  equiv[ M.swapr ~ Spec.swapr    : arg{2}.`1 = arg{1}.`1 /\ arg{2}.`2 = arg{1}.`2 /\   arg{1}.`3 = as_w64 arg{2}.`3
     ==> ={res}].
 
-declare axiom exp_ithbit :
+declare axiom iterop_ithbit :
  equiv[ M.ith_bit ~ Spec.ith_bit    : arg{2}.`1 = arg{1}.`1 /\  arg{2}.`2 = W64.to_uint arg{1}.`2 
     /\ 0 <= ctr{2} < Rsize ==> ={res} /\ (res{2} = W64.one \/ res{2} = W64.zero) ].
 
 
-declare axiom exp_mulm :
-  equiv [ M.mulm ~ Spec.mul: arg{1}.`2 = arg{2}.`1 /\ arg{1}.`3 = arg{2}.`2 /\ ImplR p{1} P /\ valR a{1} < P /\ valR b{1} < P ==> ={res} /\ valR res{1} < P  ].
+declare axiom iterop_opr :
+  equiv [ M.opr ~ Spec.mul: arg{1}.`2 = arg{2}.`1 /\ arg{1}.`3 = arg{2}.`2 /\ ImplR p{1} P /\ valR a{1} < P /\ valR b{1} < P ==> ={res} /\ valR res{1} < P  ].
 
 
 declare axiom stateless_M (x y : glob M) : x = y.
 
 
-lemma exp_real_speac :
- equiv[ M1.expm_spec ~ M7(M).expm  : valR arg{2}.`1 = P 
+lemma iterop_real_speac :
+ equiv[ M1.iterop_spec ~ M7(M).iterop  : valR arg{2}.`1 = P 
    /\  arg{1}.`1 = arg{2}.`2
    /\ bs2int arg{1}.`2 = valR arg{2}.`3
    /\ size arg{1}.`2 = Rsize
    /\ valR x{1} < P
      ==> ={res}].
-transitivity M2.expm
+transitivity M2.iterop
    (={arg} /\  0 < size arg{1}.`2  /\   valR x{1} < P  ==> ={res}) 
   (valR arg{2}.`1 = P 
    /\  arg{1}.`1 = arg{2}.`2
@@ -62,9 +62,9 @@ transitivity M2.expm
      ==> ={res} ).
 progress.  exists arg{1}. progress. smt(Rsize_pos). auto.
 symmetry.
-conseq expm_correct.
+conseq iterop_2_spec.
 auto. auto.
-transitivity M3.expm
+transitivity M3.iterop
   (={arg} /\  0 < size n{1}  ==> ={res})
   (valR arg{2}.`1 = P 
    /\  arg{1}.`1 = arg{2}.`2
@@ -74,8 +74,8 @@ transitivity M3.expm
      ==> ={res} ).
 progress. 
 exists arg{1}. progress. smt(Rsize_pos). auto.
-conseq exp_2_3.
-transitivity M4.expm
+conseq iterop_2_3.
+transitivity M4.iterop
   (arg{1}.`1 = arg{2}.`1 /\ (bitsR arg.`2{1}) = (arg.`2{2})  /\ size n{1} = Rsize /\  0 < size n{1} ==> ={res})
 (valR arg{2}.`1 = P 
    /\  arg{1}.`1 = arg{2}.`2
@@ -86,8 +86,8 @@ progress.
 exists (x{1} , ( n{2})). progress. 
 smt (bitsR_prop).
 smt(Rsize_pos). auto.
-conseq exp_3_4_1.
-transitivity M5.expm
+conseq iterop_3_4_1.
+transitivity M5.iterop
   (={arg} ==> ={res})
   (valR arg{2}.`1 = P 
    /\  arg{1}.`1 = arg{2}.`2
@@ -96,13 +96,13 @@ transitivity M5.expm
      ==> ={res} ).
 progress. 
 exists (x{1} , ( n{2})). progress.  smt(). auto.
-conseq exp_4_5.  
-transitivity M6(M).expm
+conseq iterop_4_5.  
+transitivity M6(M).iterop
  (arg{2}.`2 = arg{1}.`1 /\ arg{2}.`3 = arg{1}.`2 /\  valR m{2} = P /\ valR x{1} < P ==> ={res})
   (={arg} ==> ={res}).
 progress. smt(). smt().
-conseq (exp_5_6 M exp_swap exp_ithbit exp_mulm stateless_M).   smt().
-conseq (exp_6_7 M).
+conseq (iterop_5_6 M iterop_swap iterop_ithbit iterop_opr stateless_M).   smt().
+conseq (iterop_6_7 M).
 smt (stateless_M).
 qed.
 
